src/tls/ECGroup.fst
@@ -1,6 +1,8 @@
 module ECGroup
 module HS = FStar.HyperStack //Added automatically
 
+// cwinter: this file will likely be removed.
+
 open FStar.HyperStack
 open FStar.Bytes
 open FStar.Error
@@ -10,6 +12,7 @@ open Parse
 open FStar.HyperStack.ST
 
 module CC = CoreCrypto
+module LP = LowParse.SLow
 
 type group = CC.ec_curve
 type params = CC.ec_params
@@ -118,55 +121,74 @@ let dh_initiator #g gx gy =
     let S_CC gy = gy in
     ecdh_agreement gx gy
 
+
+// cwinter: parse_curve, parse_point, and parse_partial really describe
+// one parser for one datatype of the shape
+// { ECCurveType, ECNamedGroup (or NamedCurve), UncompressedPointRepresentation or raw bytes }
+// but I can't figure out whether that type has a name in the RFCs
+// (I don't think so, because 'namedcurve' in ECParameters only contains the 
+// curve name, no further parameters).
 val parse_curve: bytes -> Tot (option group)
 let parse_curve b =
-  if length b = 3 then
-    let (ty, id) = split b 1ul in
-    if ty.[0ul] = 3z then
-      match Parse.cbyte2 id with
-      | (0z, 23z) -> Some (ECC_P256)
-      | (0z, 24z) -> Some (ECC_P384)
-      | (0z, 25z) -> Some (ECC_P521)
-      | (0z, 29z) -> Some (ECC_X25519)
-      | (0z, 30z) -> Some (ECC_X448)
-      | _ -> None
-    else None
-  else None
+  let open Format.ECCurveType in  
+  let open Format.NamedGroup in
+  match ecCurveType_parser32 b with // <- parse_curve == ecCurveType_parser and-then named_group_parser
+  | Some (Format.ECCurveType.NAMED_CURVE, _) -> 
+      let ty, id = split b 1ul in
+      match namedGroup_parser32 id with
+      | Some (SECP256R1, _) -> Some CC.ECC_P256
+      | Some (SECP384R1, _) -> Some CC.ECC_P384
+      | Some (SECP521R1, _) -> Some CC.ECC_P521
+      | Some (X25519, _   ) -> Some CC.ECC_X25519
+      | Some (X448, _     ) -> Some CC.ECC_X448
+      | _                   -> None
+  | _ -> None
 
 val curve_id: group -> Tot (lbytes 2)
 let curve_id g =
-  twobytes (match g with
-  | ECC_P256 -> (0z, 23z)
-  | ECC_P384 -> (0z, 24z)
-  | ECC_P521 -> (0z, 25z)
-  | ECC_X25519 -> (0z, 29z)
-  | ECC_X448 -> (0z, 30z))
-
+  let open Format.NamedGroup in
+  let r = namedGroup_serializer32 ( // <- curve_id == namedGroup_serializer
+    match g with
+    | ECC_P256   -> SECP256R1
+    | ECC_P384   -> SECP384R1
+    | ECC_P521   -> SECP521R1
+    | ECC_X25519 -> X25519
+    | ECC_X448   -> X448) in
+  assume (length r = 2);
+  r
+  
 val parse_point: g:group -> bytes -> Tot (option (share g))
 let parse_point g b =
+  // parser for flat bytes or uncompressedPointPepresentation
   match g with
-  | ECC_X448 ->
-    if length b = 56 then let p : lbytes 56 = b in Some (S_X448 p)
-    else None
-  | ECC_X25519 ->
-    if length b = 32 then let p : lbytes 32 = b in Some (S_X25519 p)
-    else None
+  | ECC_X448 -> (
+      let (p:LP.parser32 _) = LP.parse32_flbytes 56 56ul in
+      match p b with
+      | Some (bs, _) -> Some (S_X448 bs)
+      | _ -> None)
+  | ECC_X25519 -> (
+      let (p:LP.parser32 _) = LP.parse32_flbytes 32 32ul in
+      match p b with
+      | Some (bs, _) -> Some (S_X25519 bs)
+      | _ -> None)
   | _ ->
-    let clen = ec_bytelen g in
-    if length b = (op_Multiply 2 clen) + 1 then
-      let (et, ecxy) = split b 1ul in
-      match et.[0ul] with
-      | 4z ->
-        let (x,y) = split_ ecxy clen in
-        let e = {ecx = x; ecy = y;} in
-        if CoreCrypto.ec_is_on_curve (params_of_group g false) e then
-          Some (S_CC e)
-        else None
-      |_ -> None
-    else None
+      let open Format.UncompressedPointRepresentation in
+      let (bl:UInt32.t) =  UInt32.uint_to_t (op_Multiply 2 (ec_bytelen g)) in
+      match (uncompressedPointRepresentation_parser32 (UInt32.v bl)) b with
+      | Some (ucpr, _) -> 
+          let e = { ecx = ucpr.x; ecy = ucpr.y } in
+          if CoreCrypto.ec_is_on_curve (params_of_group g false) e then
+            Some (S_CC e)
+          else None
+    | _ -> None
 
 val parse_partial: bytes -> Tot (result ((g:group & share g) * bytes))
 let parse_partial payload =
+    // This really means:
+    // ecCurveType_parser and-then 
+    // namedGroup_parser (or NamedCurve) and-then
+    // ( uncompressedPointRepresentation_parser or flbytes_parser )
+    // We should rewrite it using parser combinators
     if length payload >= 7 then
       let (curve, point) = split payload 3ul in
       match parse_curve curve with
@@ -187,21 +209,30 @@ val serialize_point: #g:group -> e:share g -> Tot (b:bytes{length b <= 255})
 let serialize_point #g s =
   match g with
   | ECC_X25519 ->
-    let S_X25519 p = s in p
+    let S_X25519 p = s in 
+    assert (length p = ec_bytelen g);
+    LowParse.SLow.serialize32_flbytes (ec_bytelen g) p
   | ECC_X448 ->
-    let S_X448 p = s in p
+    let S_X448 p = s in
+    assert (length p = ec_bytelen g);
+    LowParse.SLow.serialize32_flbytes (ec_bytelen g) p
   | _ ->
     let S_CC e = s in
-    let pc = abyte 4z in
-    let x = pc @| e.ecx @| e.ecy in
+    let open Format.UncompressedPointRepresentation in
+    let l = length e.ecx in
+    assert (length e.ecx = length e.ecy);
+    let ucp = { legacy_form = 4uy; x = e.ecx; y = e.ecy} in
+    let x = (uncompressedPointRepresentation_serializer32 l) ucp in
+    assert (length x = ec_bytelen g);
     x
-
+    
 val serialize: #g:group -> e:share g -> Tot (b:bytes{length b <= 259})
 let serialize #g ecdh_Y =
+  // Similar to parse_partial, we should rewrite this using serializer combinators
   let ty = abyte 3z in
   let id = curve_id g in
   let e = serialize_point ecdh_Y in
-  lemma_repr_bytes_values (length e);
+  lemma_repr_bytes_values (FStar.Bytes.length e);
   let ve = vlbytes 1 e in
   ty @| id @| ve
 
