src/tls/Format.ECCurve.fst
@@ -1,0 +1,91 @@
+module Format.ECCurve
+
+module B = FStar.Bytes
+module LP = LowParse.SLow
+module U8 = FStar.UInt8
+module U16 = FStar.UInt16
+
+open Parse.LBytes1
+
+unfold type is_injective (#a:Type) (#b:Type) (f:a -> b) 
+  = forall x y . f x == f y ==> x == y
+
+
+(* Types *)
+
+(*
+    https://tools.ietf.org/html/rfc4492#section-5.4
+
+    struct {
+        opaque a <1..2^8-1>;
+        opaque b <1..2^8-1>;
+    } ECCurve;
+
+*)
+
+noeq type ecCurve = {
+  a : lbytes_1;
+  b : lbytes_1;
+}
+
+
+(* Parsers *)
+
+let ecCurve_of_lbytes (bs:lbytes_1 * lbytes_1)
+  : Tot ecCurve
+  = let b0, b1 = bs in
+    { a = b0; b = b1 }
+
+let lbytes_of_ecCurve (c:ecCurve)
+  : Tot (lbytes_1 * lbytes_1)
+  = c.a, c.b
+
+#reset-options "--using_facts_from '* -LowParse -FStar.Reflection -FStar.Tactics' --max_fuel 16 --initial_fuel 16 --max_ifuel 16 --initial_ifuel 16"
+let lemma_ecCurve_of_lbytes_is_injective () 
+  : Lemma (is_injective ecCurve_of_lbytes) 
+  = ()
+#reset-options
+
+
+(* Parsers *)
+
+let ecCurve_parser_kind = LP.default_parser_kind
+
+let ecCurve_parser: LP.parser ecCurve_parser_kind ecCurve =
+  lemma_ecCurve_of_lbytes_is_injective ();
+  lbytes_1_parser `LP.nondep_then` lbytes_1_parser `LP.parse_synth` (fun xy -> ecCurve_of_lbytes xy)
+
+inline_for_extraction
+let ecCurve_parser32: LP.parser32 ecCurve_parser =
+  lemma_ecCurve_of_lbytes_is_injective ();
+  let pu8u8 = LP.nondep_then lbytes_1_parser lbytes_1_parser in
+  let pu8u832 = LP.parse32_nondep_then lbytes_1_parser32 lbytes_1_parser32 in
+  LP.parse32_synth pu8u8 ecCurve_of_lbytes (fun xy -> ecCurve_of_lbytes xy) pu8u832 ()
+
+
+(* Serialization *) 
+
+#reset-options "--using_facts_from '* -LowParse -FStar.Reflection -FStar.Tactics' --max_fuel 16 --initial_fuel 16 --max_ifuel 16 --initial_ifuel 16"
+let lemma_ecCurve_of_lbytes_of_ecCurve () 
+  : Lemma (forall x . ecCurve_of_lbytes (lbytes_of_ecCurve x) == x)
+  = ()
+#reset-options
+
+let ecCurve_serializer: LP.serializer ecCurve_parser = 
+  lemma_ecCurve_of_lbytes_is_injective ();
+  lemma_ecCurve_of_lbytes_of_ecCurve ();
+  let pu8u8 = LP.nondep_then lbytes_1_parser lbytes_1_parser in
+  let su8u8 = LP.serialize_nondep_then LP.parse_u8 LP.serialize_u8 () LP.parse_u8 LP.serialize_u8 in
+  LP.serialize_synth #ecCurve_parser_kind #(lbytes_1 * lbytes_1) #ecCurve
+    pu8u8 ecCurve_of_lbytes su8u8 lbytes_of_ecCurve ()
+
+inline_for_extraction
+let ecCurve_serializer32: LP.serializer32 ecCurve_serializer = 
+  lemma_ecCurve_of_lbytes_is_injective ();
+  lemma_ecCurve_of_lbytes_of_ecCurve ();
+  let pu8u8 = LP.nondep_then lbytes_1_parser lbytes_1_parser in
+  let pu8u832 = LP.parse32_nondep_then lbytes_1_parser32 lbytes_1_parser32 in
+  let su8u8 = LP.serialize_nondep_then lbytes_1_parser lbytes_1_serializer () lbytes_1_parser lbytes_1_serializer in
+  let su8u832 = LP.serialize32_nondep_then lbytes_1_serializer32 () lbytes_1_serializer32 () in
+  LP.serialize32_synth #ecCurve_parser_kind #(lbytes_1 * lbytes_1) #ecCurve
+    pu8u8 ecCurve_of_lbytes su8u8 su8u832 lbytes_of_ecCurve lbytes_of_ecCurve ()
