src/tls/Format.ECCurveType.fst
@@ -1,0 +1,99 @@
+module Format.ECCurveType
+
+module B = FStar.Bytes
+module L = FStar.List
+module U8 = FStar.UInt8
+module LP = LowParse.SLow
+
+type byte = B.byte
+
+unfold type is_injective (#a:Type) (#b:Type) (f:a -> b) 
+  = forall x y . f x == f y ==> x == y
+
+
+(* Types *)
+
+(* 
+    https://tools.ietf.org/html/rfc4492#section-5.4
+
+    enum { explicit_prime (1), explicit_char2 (2),
+           named_curve (3), reserved(248..255) } ECCurveType;
+*)
+
+noeq type ecCurveType = 
+  | EXPLICIT_PRIME
+  | EXPLICIT_CHAR2
+  | NAMED_CURVE
+  | RESERVED of (r:byte{U8.(248uy <=^ r && r <=^ 255uy)})
+  | UNKNOWN of (r:byte{not U8.(248uy <=^ r && r <=^ 255uy) /\
+                       not U8.(r =^ 1uy) /\
+                       not U8.(r =^ 2uy) /\
+                       not U8.(r =^ 3uy)})
+
+inline_for_extraction
+let ecCurveType_of_byte (b:byte)
+  : Tot ecCurveType
+  = match b with
+  | 0x01uy -> EXPLICIT_PRIME
+  | 0x02uy -> EXPLICIT_CHAR2
+  | 0x03uy -> NAMED_CURVE
+  | r      -> if U8.lt 248uy r && U8.lt r 255uy then RESERVED r 
+              else UNKNOWN r
+
+inline_for_extraction
+let byte_of_ecCurveType (c:ecCurveType)
+  : byte
+  = match c with
+  | EXPLICIT_PRIME -> 0x01uy
+  | EXPLICIT_CHAR2 -> 0x02uy
+  | NAMED_CURVE    -> 0x03uy
+  | RESERVED r     -> r
+  | UNKNOWN r      -> r
+
+let is_named (t:ecCurveType): Tot bool = t = NAMED_CURVE
+
+#reset-options "--using_facts_from '* -LowParse -FStar.Reflection -FStar.Tactics' --max_fuel 16 --initial_fuel 16 --max_ifuel 16 --initial_ifuel 16"
+let lemma_ecCurveType_of_byte_is_injective () 
+  : Lemma (is_injective ecCurveType_of_byte) 
+  = ()
+#reset-options
+
+
+(* Parsers *)
+
+let ecCurveType_parser_kind = LP.parse_u8_kind
+
+let ecCurveType_parser: LP.parser ecCurveType_parser_kind ecCurveType =
+  lemma_ecCurveType_of_byte_is_injective ();
+  LP.parse_u8 `LP.parse_synth` ecCurveType_of_byte 
+
+inline_for_extraction
+let ecCurveType_parser32: LP.parser32 ecCurveType_parser =
+  lemma_ecCurveType_of_byte_is_injective ();
+  LP.parse32_synth LP.parse_u8 ecCurveType_of_byte (fun x -> ecCurveType_of_byte x) LP.parse32_u8 ()
+
+
+// (* Validators? *)
+
+
+// (* Serialization *) 
+
+#reset-options "--using_facts_from '* -LowParse -FStar.Reflection -FStar.Tactics' --max_fuel 16 --initial_fuel 16 --max_ifuel 16 --initial_ifuel 16"
+let lemma_ecCurveType_of_byte_of_ecCurveType () 
+  : Lemma (forall x . ecCurveType_of_byte (byte_of_ecCurveType x) == x)
+  = ()
+#reset-options
+
+let ecCurveType_serializer: LP.serializer ecCurveType_parser = 
+  lemma_ecCurveType_of_byte_is_injective ();
+  lemma_ecCurveType_of_byte_of_ecCurveType ();
+  LP.serialize_synth #ecCurveType_parser_kind #byte #ecCurveType
+    LP.parse_u8 ecCurveType_of_byte LP.serialize_u8 byte_of_ecCurveType ()
+
+inline_for_extraction
+let ecCurveType_serializer32: LP.serializer32 ecCurveType_serializer = 
+  lemma_ecCurveType_of_byte_is_injective ();
+  lemma_ecCurveType_of_byte_of_ecCurveType ();
+  LP.serialize32_synth #ecCurveType_parser_kind #byte #ecCurveType
+    LP.parse_u8 ecCurveType_of_byte LP.serialize_u8 LP.serialize32_u8 byte_of_ecCurveType (fun x -> byte_of_ecCurveType x) ()
+
