src/tls/Format.LByte1.fst
@@ -1,0 +1,67 @@
+module Format.LBytes1
+
+module B = FStar.Bytes
+module LP = LowParse.SLow
+
+unfold type is_injective (#a:Type) (#b:Type) (f:a -> b) 
+  = forall x y . f x == f y ==> x == y
+
+
+(* 
+   Frequently used 
+
+   opaque x<1..2^8-1> 
+*)
+
+
+(* Types *)
+
+let is_lbytes_1 (b:bytes) = 0 < B.length b && B.length b < 256
+
+type lbytes_1 = b:bytes{is_lbytes_1 b}
+
+
+(* Parsers *)
+
+inline_for_extraction 
+let lbytes_1_of_bytes (b:bytes{is_lbytes_1 b}): Tot lbytes_1 = b
+
+inline_for_extraction
+let bytes_of_lbytes_1 (p:lbytes_1): Tot lbytes_1 = p
+
+let lemma_lbytes_1_of_bytes_is_injective () 
+  : Lemma (is_injective lbytes_1_of_bytes) 
+  = ()
+
+let lbytes_1_parser_kind = LP.parse_bounded_vldata_kind 1 255
+
+let lbytes_1_parser
+  : LP.parser lbytes_1_parser_kind lbytes_1 
+  = lemma_lbytes_1_of_bytes_is_injective ();
+    LP.parse_bounded_vldata 1 255 LP.parse_u8
+
+inline_for_extraction 
+let lbytes_1_parser32
+  : LP.parser32 lbytes_1_parser 
+  = lemma_lbytes_1_of_bytes_is_injective ();
+    LP.parse32_bounded_vldata 1 1ul 255 255ul LP.parse32_u8
+
+
+(* Serialization *)
+
+let lemma_lbytes_1_of_bytes_of_lbytes_1 () 
+  : Lemma (forall x . lbytes_1_of_bytes (bytes_of_lbytes_1 x) == x)
+  = ()
+
+let lbytes_1_serializer
+  : LP.serializer lbytes_1_parser 
+  = lemma_lbytes_1_of_bytes_is_injective ();
+    lemma_lbytes_1_of_bytes_of_lbytes_1 ();
+    LP.serialize_bounded_vldata_strong 1 255 LP.serialize_u8
+
+inline_for_extraction 
+let lbytes_1_serializer32
+  : LP.serializer32 lbytes_1_serializer 
+  = lemma_lbytes_1_of_bytes_is_injective ();
+    lemma_lbytes_1_of_bytes_of_lbytes_1 ();
+    LP.serialize32_bounded_vldata_strong 1 255 LP.serialize32_u8
