src/tls/Format.NamedGroupList.fst
@@ -1,7 +1,6 @@
-module Parse.NamedGroups
+module Format.NamedGroupList
 
-open Parse.Lemmas
-open Parse.NamedGroup
+open Format.NamedGroup
 
 module LP = LowParse.SLow
 module L = FStar.List.Tot
@@ -12,77 +11,75 @@ module L = FStar.List.Tot
 (* https://tlswg.github.io/tls13-spec/draft-ietf-tls-tls13.html#rfc.section.4.2.7
 
     struct {
-        NamedGroup named_group_list<2..2^16-1>;
+        NamedGroup namedGroup_list<2..2^16-1>;
     } NamedGroupList;
            
 *)
 
-type named_groups = l:list named_group {1 <= L.length l && L.length l <= 32767}
+type namedGroupList = l:list namedGroup {1 <= L.length l && L.length l <= 32767}
+
+let bytesize (gs:namedGroupList): Tot nat = 2 + (op_Multiply Format.NamedGroup.bytesize (L.length gs))
 
 private
-let bytesize (gs:named_groups) = 2 + (op_Multiply named_group_bytesize (L.length gs))
-
-private
-let nglist_serializer = LP.serialize_list _ named_group_serializer
-
+let nglist_serializer = LP.serialize_list _ namedGroup_serializer
 
 inline_for_extraction
-let synth_named_groups
+let synth_namedGroupList
   (l:LP.parse_bounded_vldata_strong_t 2 65535 nglist_serializer)
-  : Tot (l:named_groups)
+  : Tot (l:namedGroupList)
   = [@inline_let]
-    let l' : list named_group = l in
+    let l' : list namedGroup = l in
     [@inline_let]
     let _ = assume (1 <= L.length l' /\ L.length l' <= 32767) in
     l'
 
 inline_for_extraction
-let synth_named_groups_recip
-  (l:named_groups)
+let synth_namedGroupList_recip
+  (l:namedGroupList)
   : Tot (l:LP.parse_bounded_vldata_strong_t 2 65535 nglist_serializer)
   = [@inline_let]
-    let l' : list named_group = l in
+    let l' : list namedGroup = l in
     [@inline_let]
     let _ = assume (LP.parse_bounded_vldata_strong_pred 2 65535 nglist_serializer l') in
     l'
 
 (* Parsers *)
 
-let named_groups_parser_kind = LP.parse_bounded_vldata_kind 2 65535
+let namedGroupList_parser_kind = LP.parse_bounded_vldata_kind 2 65535
 
-let named_groups_parser: LP.parser named_groups_parser_kind _ =
+let namedGroupList_parser: LP.parser namedGroupList_parser_kind _ =
   LP.parse_synth
     (LP.parse_bounded_vldata_strong 2 65535 nglist_serializer)
-    synth_named_groups
+    synth_namedGroupList
 
 inline_for_extraction
-let named_groups_parser32: LP.parser32 named_groups_parser =
+let namedGroupList_parser32: LP.parser32 namedGroupList_parser =
   LP.parse32_synth
     _
-    synth_named_groups
-    (fun x -> synth_named_groups x)
-    (LP.parse32_bounded_vldata_strong 2 2ul 65535 65535ul nglist_serializer (LP.parse32_list named_group_parser32))
+    synth_namedGroupList
+    (fun x -> synth_namedGroupList x)
+    (LP.parse32_bounded_vldata_strong 2 2ul 65535 65535ul nglist_serializer (LP.parse32_list namedGroup_parser32))
     ()
 
 
 (* Serialization *) 
 
-let named_groups_serializer: LP.serializer named_groups_parser =
+let namedGroupList_serializer: LP.serializer namedGroupList_parser =
   LP.serialize_synth
     _
-    synth_named_groups
-    (LP.serialize_bounded_vldata_strong 2 65535 (LP.serialize_list named_group_parser named_group_serializer))
-    synth_named_groups_recip
+    synth_namedGroupList
+    (LP.serialize_bounded_vldata_strong 2 65535 (LP.serialize_list namedGroup_parser namedGroup_serializer))
+    synth_namedGroupList_recip
     ()
 
 inline_for_extraction
-let named_groups_serializer32: LP.serializer32 named_groups_serializer =
+let namedGroupList_serializer32: LP.serializer32 namedGroupList_serializer =
   LP.serialize32_synth
     _
-    synth_named_groups
+    synth_namedGroupList
     _
     (LP.serialize32_bounded_vldata_strong 2 65535
-      (LP.partial_serialize32_list _ named_group_serializer named_group_serializer32 ()))
-    synth_named_groups_recip
-    (fun x -> synth_named_groups_recip x)
+      (LP.partial_serialize32_list _ namedGroup_serializer namedGroup_serializer32 ()))
+    synth_namedGroupList_recip
+    (fun x -> synth_namedGroupList_recip x)
     ()
